Finished Stack.ADT

common/StackADT.v
@@ -204,16 +204,6 @@ Proof.
   rewrite map_app, concat_app, in_app; tauto.
 Qed.
 
-(* Lemma in_frames_app: *)
-(*   forall l1 l2 b, *)
-(*     in_frames l1 b \/ in_frames l2 b <-> *)
-(*     in_frames (l1 ++ l2) b. *)
-(* Proof. *)
-(*   intros. *)
-(*   unfold in_frames, get_frames_blocks in *. *)
-(*   rewrite map_app, concat_app, in_app; tauto. *)
-(* Qed. *)
-
 Lemma in_frame_info:
   forall b (f: frame_adt),
     in_frame f b ->
@@ -734,51 +724,36 @@ Section INJ.
      eapply frame_inject_compose; eauto.
    Qed.
 
-   Inductive stack_inject_aux (f: meminj) (m: perm_type) : frameinj -> stack -> stack -> Prop :=
-   | stack_inject_aux_intro:
-       stack_inject_aux f m nil nil nil
-   | stack_inject_aux_cons
+   Inductive stack_inject (f: meminj) (m: perm_type) : frameinj -> stack -> stack -> Prop :=
+   | stack_inject_intro:
+       stack_inject f m nil nil nil
+   | stack_inject_cons
        n g s1 hs1 ts1 tf ts2
        (TAKE: take (S n) s1 = Some hs1)
        (DROP: drop (S n) s1 = ts1)
-       (SIA_REC: stack_inject_aux f m g ts1 ts2)
+       (SIA_REC: stack_inject f m g ts1 ts2)
        (FI: Forall (fun f1 => tframe_inject f m f1 tf) hs1):
-     stack_inject_aux f m (S n::g) s1 (tf::ts2).
+     stack_inject f m (S n::g) s1 (tf::ts2).
 
-   Lemma stack_inject_aux_length_l:
+   Lemma stack_inject_length_l:
      forall f m g s1 s2,
-       stack_inject_aux f m g s1 s2 ->
+       stack_inject f m g s1 s2 ->
        sum_list g = length s1.
    Proof.
      induction 1; simpl; intros; eauto.
      rewrite (take_drop _ _ _ TAKE). subst.
-     rewrite IHstack_inject_aux. rewrite app_length.
+     rewrite IHstack_inject. rewrite app_length.
      f_equal. symmetry.
      erewrite take_length by eauto. omega.
    Qed.
 
-   Lemma stack_inject_aux_length_r:
+   Lemma stack_inject_length_r:
      forall f m g s1 s2,
-       stack_inject_aux f m g s1 s2 ->
+       stack_inject f m g s1 s2 ->
        length g = length s2.
    Proof.
      induction 1; simpl; intros; eauto.
    Qed.
-
-   Record stack_inject (f: meminj) (g: frameinj) (m: perm_type) (s1 s2: stack) :=
-    {
-      (* stack_src_wf: wf_stack m s1; *)
-      stack_inject_frame_inject: stack_inject_aux f m g s1 s2;
-      stack_inject_not_in_source:
-        forall b1 b2 delta bi2
-          (FB: f b1 = Some (b2, delta))
-          (NIS: ~ in_stack s1 b1)
-          (FI: in_stack' s2 (b2,bi2))
-          o k p
-          (PERM: m b1 o k p)
-          (IPC: inject_perm_condition p),
-          frame_public bi2 (o + delta);
-    }.
 
   Lemma concat_In:
     forall {A} (l: list (list A)) b,
@@ -821,7 +796,7 @@ Section INJ.
 
   Lemma stack_inject_compat:
     forall f g P s1 s2,
-      stack_inject f g P s1 s2 ->
+      stack_inject f P g s1 s2 ->
     forall b1 b2 delta bi1,
       f b1 = Some (b2, delta) ->
       in_stack' s1 (b1, bi1) ->
@@ -830,9 +805,7 @@ Section INJ.
         in_stack' s2 (b2, bi2) /\ inject_frame_info delta bi1 bi2.
   Proof.
     intros f g P s1 s2 SI.
-    inv SI.
-    revert stack_inject_frame_inject0 .
-    clear stack_inject_not_in_source0.
+    revert SI.
     induction 1; simpl; intros b1 b2 delta bi1 FB INS PERM.
     - easy.
     - subst.
@@ -855,7 +828,7 @@ Section INJ.
         destruct FI as (bi2 & INfr2 & IFI).
         exists bi2; split; auto. left; rewrite in_frames'_rew.
         eexists; split; eauto.
-      + edestruct IHstack_inject_frame_inject0 as (bi2 & INS2 & IFI); eauto.
+      + edestruct IHSI as (bi2 & INS2 & IFI); eauto.
   Qed.
 
   Lemma stack_top_in_frames:
@@ -900,7 +873,7 @@ Section INJ.
 
   Lemma stack_inject_is_stack_top:
     forall f g m s1 s2,
-      stack_inject f g m s1 s2 ->
+      stack_inject f m g s1 s2 ->
       forall b1 b2 delta,
         f b1 = Some (b2, delta) ->
         (exists o k p, m b1 o k p /\ inject_perm_condition p) ->
@@ -910,7 +883,7 @@ Section INJ.
     intros f g m s1 s2 SI b1 b2 delta FB PERM IST.
     destruct (stack_top_frame_at_position _ _ IST) as (ff & FAP1 & IFR1).
     destruct s1. inv FAP1. simpl in *. congruence.
-    inv SI. inv stack_inject_frame_inject0.
+    inv SI.
     eapply frame_at_position_stack_top; eauto.
     constructor. reflexivity.
     inv FAP1. inv H.
@@ -976,37 +949,6 @@ Section INJ.
       exfalso; eapply H6. eauto. eapply in_frames_in_stack; eauto.
       inv H. eapply IHl; eauto.
   Qed.
-
-  (* Inductive nodupt: tframe_adt -> Prop := *)
-  (* | nodupt_nil: nodupt nil *)
-  (* | nodupt_cons: forall f s, nodupt s -> (forall b, in_frame f b -> ~ in_frames s b) -> nodupt (f::s). *)
-
-  (* Definition nodupt (s: tframe_adt) := *)
-  (*   forall b f1 f2, *)
-  (*     In f1 s -> *)
-  (*     In f2 s -> *)
-  (*     in_frame f1 b -> *)
-  (*     in_frame f2 b -> *)
-  (*     f1 = f2. *)
-
-
-  (* Lemma nodupt_nodupt': forall l, nodupt l -> nodupt' l. *)
-  (* Proof. *)
-  (*   induction 1; simpl; intros; eauto. *)
-  (*   - unfold nodupt'. easy. *)
-  (*   - intros b f1 f2 [EQ1|AIN1] [EQ2|AIN2] IFR1 IFR2; subst; simpl in *; auto. *)
-  (*     + eapply H0 in IFR1. elim IFR1. *)
-  (*       unfold in_frames, get_frames_blocks. *)
-  (*       apply concat_In. *)
-  (*       eexists; split. apply IFR2. *)
-  (*       apply in_map. simpl. auto. *)
-  (*     + eapply H0 in IFR2. elim IFR2. *)
-  (*       unfold in_frames, get_frames_blocks. *)
-  (*       apply concat_In. *)
-  (*       eexists; split. apply IFR1. *)
-  (*       apply in_map. simpl. auto. *)
-  (*     + eapply IHnodupt; eauto. *)
-  (* Qed. *)
 
   Lemma in_frames_in_frame_ex:
     forall tf b,
@@ -1201,7 +1143,7 @@ Section INJ.
 
   Lemma stack_inject_inject_frame_info:
     forall f g m l1 l2,
-      stack_inject f g m l1 l2 ->
+      stack_inject f m g l1 l2 ->
       nodup l1 ->
       nodup l2 ->
       forall b1 bi1 b2 bi2,
@@ -1244,14 +1186,14 @@ Section INJ.
       drop n1 (drop n2 l) = drop (n1 + n2) l.
   Proof.
     induction n1; simpl; intros; eauto.
-    rewrite <- IHn1. rewrite drop_tl. auto.
+    rewrite <- IHn1. rewrite drop_tl. reflexivity.
   Qed.
 
   Lemma stack_inject_drop:
     forall f m1 g1 l1 l2
-      (SI : stack_inject_aux f m1 g1 l1 l2)
+      (SI : stack_inject f m1 g1 l1 l2)
       n (POS: O < n) l (TAKE : take n g1 = Some l),
-      stack_inject_aux f m1 (drop n g1) (drop (sum_list l) l1) (drop n l2).
+      stack_inject f m1 (drop n g1) (drop (sum_list l) l1) (drop n l2).
   Proof.
     induction 1; simpl; intros; eauto.
     - destruct n; simpl in *; inv TAKE. simpl. constructor.
@@ -1283,15 +1225,15 @@ Section INJ.
     repeat destr_in H. simpl. eauto.
   Qed.
 
-  Lemma stack_inject_aux_take:
+  Lemma stack_inject_take:
     forall n
       f m g s1 s2
-      (SIA: stack_inject_aux f m g s1 s2)
+      (SIA: stack_inject f m g s1 s2)
       g' s1' s2'
       (TG: take n g = Some g')
       (TS1: take (sum_list g') s1 = Some s1')
       (TS2: take n s2 = Some s2'),
-      stack_inject_aux f m g' s1' s2'.
+      stack_inject f m g' s1' s2'.
   Proof.
     induction n; simpl; intros.
     - inv TG; inv TS2. simpl in *. inv TS1. constructor.
@@ -1302,9 +1244,9 @@ Section INJ.
       eapply take_drop_rest; eauto.
   Qed.
 
-  Lemma stack_inject_aux_tframe_inject:
+  Lemma stack_inject_tframe_inject:
     forall f m g s1 s2 x,
-      stack_inject_aux f m g s1 s2 ->
+      stack_inject f m g s1 s2 ->
       In x s1 ->
       exists y, In y s2 /\ tframe_inject f m x y.
   Proof.
@@ -1313,23 +1255,23 @@ Section INJ.
     rewrite (take_drop _ _ _ TAKE) in H0. rewrite in_app in H0.
     destruct H0.
     rewrite Forall_forall in FI. apply FI in H0. eauto.
-    destruct IHstack_inject_aux as (y & INs2 & TFI). auto.
+    destruct IHstack_inject as (y & INs2 & TFI). auto.
     eauto.
   Qed.
 
   Opaque take drop.
 
-  Lemma stack_inject_aux_compose:
+  Lemma stack_inject_compose_aux:
     forall f f' m1 m2 g1 g2 s1 s2 s3 g3
       (COMP : compose_frameinj g1 g2 = Some g3)
-      (SI12 : stack_inject_aux f m1 g1 s1 s2)
-      (SI23 : stack_inject_aux f' m2 g2 s2 s3)
+      (SI12 : stack_inject f m1 g1 s1 s2)
+      (SI23 : stack_inject f' m2 g2 s2 s3)
       (PERMS: forall b1 b2 delta o k p,
           f b1 = Some (b2, delta) ->
           m1 b1 o k p ->
           inject_perm_condition p ->
           m2 b2 (o + delta)%Z k p),
-      stack_inject_aux (compose_meminj f f') m1 g3 s1 s3.
+      stack_inject (compose_meminj f f') m1 g3 s1 s3.
   Proof.
     intros.
     revert f' m2 g2 s2 s3 SI23 f m1 g1 s1 SI12 g3 COMP PERMS.
@@ -1338,7 +1280,7 @@ Section INJ.
     - repeat destr_in COMP.
       repeat destr_in H0. repeat destr_in Heqo. simpl in *.
       destruct (take_succeeds (sum_list l) s0) as (t & EQ).
-      erewrite <- stack_inject_aux_length_l by eauto.
+      erewrite <- stack_inject_length_l by eauto.
       eapply take_sumlist; eauto.
       cut (exists sl, sum_list l = S sl). intros (sl & SL). rewrite SL in *.
       econstructor; eauto.
@@ -1346,9 +1288,9 @@ Section INJ.
       rewrite <- SL.
       eapply stack_inject_drop; eauto. omega.
       rewrite Forall_forall in FI |- *. intros.
-      exploit stack_inject_aux_take. apply SI12. eauto. rewrite SL; eauto. eauto. 
+      exploit stack_inject_take. apply SI12. eauto. rewrite SL; eauto. eauto. 
       intro SIA.
-      edestruct (stack_inject_aux_tframe_inject _ _ _ _ _ x SIA) as (y & INhs1 & TFI). auto.
+      edestruct (stack_inject_tframe_inject _ _ _ _ _ x SIA) as (y & INhs1 & TFI). auto.
       eapply tframe_inject_compose; eauto.
       Transparent take drop.
       inv SI12; simpl in *. congruence.
@@ -1357,9 +1299,9 @@ Section INJ.
 
   Lemma stack_inject_compose:
     forall (f f' : meminj) g g' m1 l1 l2,
-      stack_inject f g m1 l1 l2 ->
+      stack_inject f m1 g l1 l2 ->
       forall m2 l3,
-        stack_inject f' g' m2 l2 l3 ->
+        stack_inject f' m2 g' l2 l3 ->
         nodup l2 ->
         nodup l3 ->
         (forall b1 b2 delta o k p,
@@ -1370,84 +1312,26 @@ Section INJ.
         stack_agree_perms m2 l2 ->
         forall g3,
         (compose_frameinj g g') = Some g3 ->
-        stack_inject (compose_meminj f f') g3 m1 l1 l3.
+        stack_inject (compose_meminj f f') m1 g3 l1 l3.
   Proof.
     intros f f' g g' m1 l1 l2 SI1 m2 l3 SI2 ND2 ND3 PERM FAP g3 COMP.
-    inversion SI1; inversion SI2.
-    split; auto.
-    - eapply stack_inject_aux_compose; eauto.
-    - intros b1 b3 delta bi3 CINJ NIS1 INS3 o k p PERMS IPC.
-      unfold compose_meminj in CINJ.
-      destruct (f b1) as [[b2 delta1]|] eqn:FB1; try congruence.
-      destruct (f' b2) as [[b33 delta2]|] eqn:FB2; try congruence.
-      inv CINJ.
-      destruct (in_stack_dec l2 b2).
-      +
-        assert (INS2: exists bi2, in_stack' l2 (b2,bi2)).
-        {
-          destruct (in_stack_in_frames_ex _ _ i) as (f2 & INS2 & INF2).
-          setoid_rewrite in_stack'_rew.
-          edestruct in_frames_in_frame_ex as (f2' & INS2' & INF2'). apply INF2.
-          edestruct in_frame_info as (bi2 & IFR2). apply INF2'.
-          setoid_rewrite in_frames'_rew.
-          exists bi2, f2. split; auto.
-          exists f2'; split; auto.
-        }
-        destruct INS2 as (bi2 & INS2).
-        exploit stack_inject_not_in_source0. eauto. eauto. eauto. eauto. auto.
-        intro PUB2.
-        exploit PERM; eauto. intro PERMS2.
-        rewrite Z.add_assoc. eapply public_stack_shift; eauto.
-        2: eapply in_stack'_stack_agree_perms; eauto.
-        eapply stack_inject_inject_frame_info; eauto.
-      + rewrite Z.add_assoc. eapply stack_inject_not_in_source1; eauto.
+    eapply stack_inject_compose_aux; eauto.
   Qed.
 
-  Definition public_stack_access l (b: block) (lo hi: Z) : Prop :=
-    match get_frame_info l b with
-      Some fi => public_stack_range lo hi fi
-    | None => True
-    end.
-
-  Lemma lo_ge_hi_public_stack_access:
-    forall m b lo hi,
-      (lo >= hi)%Z ->
-      public_stack_access m b lo hi.
-  Proof.
-    red. intros.
-    destruct (get_frame_info m b); try tauto.
-    red; intros. omega.
-  Qed.
-
-  Definition stack_access (m: stack) (b: block) (lo hi: Z) : Prop :=
-    is_stack_top m b \/ public_stack_access m b lo hi.
-
-  Lemma is_stack_top_dec : forall m b,
-      {is_stack_top m b} + {~is_stack_top m b}.
+  Lemma is_stack_top_dec : forall s b,
+      {is_stack_top s b} + {~is_stack_top s b}.
   Proof.
     intros. unfold is_stack_top. apply in_dec. 
     apply eq_block.
   Qed.
 
-  Lemma lo_ge_hi_stack_access:
-    forall m b lo hi,
-      (lo >= hi)%Z ->
-      stack_access m b lo hi.
-  Proof.
-    unfold stack_access.
-    intros.
-    destruct (is_stack_top_dec m b);[left|right]. auto.
-    eapply lo_ge_hi_public_stack_access. auto.
-  Qed.
-
-
   Lemma is_stack_top_stack_blocks:
-    forall m b,
-      is_stack_top m b <-> (exists f r, in_frames f b /\ m = f::r).
+    forall s b,
+      is_stack_top s b <-> (exists f r, in_frames f b /\ s = f::r).
   Proof.
     unfold is_stack_top, get_stack_top_blocks.
     intros.
-    destruct m eqn:?; intuition.
+    destruct s eqn:?; intuition.
     - decompose [ex and] H; intuition congruence.
     - repeat eexists. eauto.
     - subst.    
@@ -1455,82 +1339,13 @@ Section INJ.
       eauto. 
   Qed.
 
-  Lemma in_stack_data_inside:
-    forall fi lo hi lo' hi',
-      public_stack_range lo hi fi ->
-      (lo <= lo')%Z ->
-      (hi' <= hi)%Z ->
-      public_stack_range lo' hi' fi.
-  Proof.
-    intros fi lo hi lo' hi' NPSA LO HI.
-    do 2 red in NPSA |- *.
-    intros; apply NPSA. omega.
-  Qed.
-
-  Lemma public_stack_access_inside:
-    forall m b lo hi lo' hi',
-      public_stack_access m b lo hi ->
-      (lo <= lo')%Z ->
-      (hi' <= hi)%Z ->
-      public_stack_access m b lo' hi'.
-  Proof.
-    intros m b lo hi lo' hi' NPSA LO HI.
-    unfold public_stack_access in *.
-    destruct (get_frame_info m b); auto.
-    eapply in_stack_data_inside in NPSA; eauto.
-  Qed.
-
-  Lemma stack_access_inside:
-    forall m b lo hi lo' hi',
-      stack_access m b lo hi ->
-      (lo <= lo')%Z ->
-      (hi' <= hi)%Z ->
-      stack_access m b lo' hi'.
-  Proof.
-    intros m b lo hi lo' hi' NPSA LO HI.
-    unfold stack_access in *.
-    destruct NPSA; auto. right.
-    eapply public_stack_access_inside; eauto.
-  Qed.
-
-  Lemma public_stack_range_dec : forall lo hi f,
-      {public_stack_range lo hi f} + {~public_stack_range lo hi f}.
-  Proof.
-    unfold public_stack_range. intros. 
-    edestruct (Intv.forall_rec (frame_public f) (fun ofs => ~ frame_public f ofs)) with (lo:=lo) (hi:=hi).
-    - apply frame_public_dec. 
-    - auto.
-    - right. intro A.
-      destruct e as (x & IN & NIN).
-      apply NIN. apply A. auto.
-  Qed.
-
-  Lemma public_stack_access_dec : forall m b lo hi,
-      {public_stack_access m b lo hi} + 
-      {~public_stack_access m b lo hi}.
-  Proof.
-    unfold public_stack_access.
-    intros.
-    destruct (get_frame_info m b); auto.
-    apply public_stack_range_dec.
-  Qed.
-
-  Lemma stack_access_dec : forall m b lo hi,
-      {stack_access m b lo hi} + 
-      {~stack_access m b lo hi}.
-  Proof.
-    intros. unfold stack_access.
-    destruct (is_stack_top_dec m b); auto.
-    destruct (public_stack_access_dec m b lo hi); auto.
-    right; intuition.
-  Qed.
-
-
   Lemma not_in_frames_no_frame_info:
-    forall (m : tframe_adt) (b : block), ~ in_frames m b -> get_assoc_tframes m b = None.
+    forall (tf : tframe_adt) (b : block), 
+      ~ in_frames tf b -> 
+      get_assoc_tframes tf b = None.
   Proof.
     intros.
-    destruct (get_assoc_tframes m b) eqn:GAT; auto.
+    destruct (get_assoc_tframes tf b) eqn:GAT; auto.
     apply get_assoc_tframes_in in GAT.
     destruct GAT as (f0 & IN1 & IN2).
     exfalso; apply H.
@@ -1539,18 +1354,18 @@ Section INJ.
   Qed.
 
   Lemma get_frame_info_in_frames:
-    forall m b f, get_assoc_tframes m b = Some f -> in_frames m b.
+    forall tf b f, get_assoc_tframes tf b = Some f -> in_frames tf b.
   Proof.
     intros.
-    destruct (in_frames_dec m b); auto.
+    destruct (in_frames_dec tf b); auto.
     rewrite not_in_frames_no_frame_info in H; auto. congruence.
   Qed.
 
   Lemma get_frame_info_in_stack:
-    forall m b f, get_frame_info m b = Some f -> in_stack m b.
+    forall s b f, get_frame_info s b = Some f -> in_stack s b.
   Proof.
     intros.
-    destruct (in_stack_dec m b); auto.
+    destruct (in_stack_dec s b); auto.
     rewrite not_in_stack_get_assoc in H; auto. congruence.
   Qed.
 
@@ -1586,7 +1401,7 @@ Section INJ.
   Lemma in_frame_get_assoc:
     forall a b,
       in_frame a b ->
-      exists f : frame_info, get_assoc positive frame_info peq (frame_adt_blocks a) b = Some f.
+      exists fi : frame_info, get_assoc positive frame_info peq (frame_adt_blocks a) b = Some fi.
   Proof.
     unfold in_frame, get_frame_blocks.
     intros a.
@@ -1599,7 +1414,7 @@ Section INJ.
   Lemma in_frames_get_assoc_tframes:
     forall s b,
       in_frames s b ->
-      exists f, get_assoc_tframes s b = Some f.
+      exists fi, get_assoc_tframes s b = Some fi.
   Proof.
     unfold in_frames, get_assoc_tframes. intros. destr; try easy.
     rewrite pred_dec_true.
@@ -1609,7 +1424,7 @@ Section INJ.
   Lemma in_stack_get_assoc_stack:
     forall s b,
       in_stack s b ->
-      exists f, get_assoc_stack s b = Some f.
+      exists fi, get_assoc_stack s b = Some fi.
   Proof.
     induction s; simpl; intros; eauto. easy.
     rewrite in_stack_cons in H.
@@ -1620,16 +1435,12 @@ Section INJ.
 
   Lemma get_frame_info_inj_gen:
     forall f g m1 s1 s2 b1 b2 delta
-      (SI: stack_inject f g m1 s1 s2)
+      (SI: stack_inject f m1 g s1 s2)
       (ND1: nodup s1)
       (ND2: nodup s2)
       (FB : f b1 = Some (b2, delta))
       (PERM: exists o k p, m1 b1 o k p /\ inject_perm_condition p),
-      option_le_stack (fun fi => 
-                   forall ofs k p,
-                     m1 b1 ofs k p ->
-                     inject_perm_condition p ->
-                     frame_public fi (ofs + delta))
+      option_le_stack (fun fi => True) (* this correct? *)
                 (inject_frame_info delta)
                 delta
                 (get_frame_info s1 b1)
@@ -1659,15 +1470,12 @@ Section INJ.
       destruct (get_assoc_stack s2 b2) eqn:FI2.
       + apply option_le_none_some.
         edestruct get_assoc_spec as (fr & tfr & IN & AIN & INR); eauto.
-        intros; eapply stack_inject_not_in_source; eauto.
-        rewrite in_stack'_rew. setoid_rewrite in_frames'_rew.
-        exists tfr. split. exists fr; split; auto. auto.
       + apply option_le_none_none.
   Qed.
 
   Lemma is_stack_top_inj_gen:
     forall P f g s1 s2 b1 b2 delta
-      (MINJ: stack_inject f g P s1 s2)
+      (MINJ: stack_inject f P g s1 s2)
       (FB: f b1 = Some (b2, delta))
       (PERM: exists o k p, P b1 o k p /\ inject_perm_condition p)
       (IST: is_stack_top s1 b1),
@@ -1675,61 +1483,6 @@ Section INJ.
   Proof.
     intros.
     eapply stack_inject_is_stack_top; eauto.
-  Qed.
-
-  Lemma stack_access_inj_gen:
-    forall f g m1 s1 s2 b1 b2 delta lo hi p
-      (MINJ : stack_inject f g m1 s1 s2)
-      (ND1: nodup s1)
-      (ND2: nodup s2)
-      (FAP: stack_agree_perms m1 s1)
-      (FB : f b1 = Some (b2, delta))
-      (RP: forall o, (lo <= o < hi)%Z -> m1 b1 o Cur p)
-      (IPC: inject_perm_condition p)
-      (NPSA: stack_access s1 b1 lo hi),
-      stack_access s2 b2 (lo + delta) (hi + delta).
-  Proof.
-    unfold stack_access, public_stack_access.
-    intros. revert NPSA.
-    destruct (zlt lo hi).
-    intros [A|A].
-    - exploit is_stack_top_inj_gen; eauto.
-      exists lo, Cur, p; split; eauto. apply RP. omega.
-    - assert (forall fi, get_frame_info s2 b2 = Some fi -> public_stack_range (lo+delta) (hi+delta) fi).
-      {
-        intros.
-        assert (in_stack s2 b2).
-        exploit get_assoc_spec. eauto. intros (fr & tf & IN1 & AIN & IN2).
-        eapply in_frames_in_stack; eauto.
-        eapply in_frame_in_frames; eauto.
-        eapply in_frame_blocks_in_frame; eauto.
-        generalize (get_frame_info_inj_gen _ _ _ _ _ _ _ _ MINJ ND1 ND2 FB). rewrite H. intro GFIJ.
-        trim GFIJ.
-        {
-          exists lo, Cur, p; split; eauto. apply RP; omega.
-        }
-        inv GFIJ.
-        - rewrite <- H1 in A.
-          symmetry in H1. apply get_assoc_spec in H1.
-          destruct H1 as (fr & tf & IN1 & AIN & IN2).
-          specialize (FAP _ IN2 _ AIN).
-          red in FAP.
-          assert (forall o, lo <= o < hi -> 0 <= o < frame_size a)%Z as INFR.
-          intros.
-          eapply FAP. eauto. apply RP. auto.
-          destruct (zlt lo hi).
-          + eapply public_stack_range_shift; eauto.
-            apply INFR; auto. omega.
-            cut (hi - 1 < frame_size a)%Z. omega.
-            apply INFR; auto. omega.
-          + eapply public_stack_range_lo_ge_hi. omega.
-        - red.  intros.
-          replace ofs with (ofs-delta+delta)%Z by omega. eapply H3.
-          apply RP. omega. auto.
-      }     
-      right; destr.
-      specialize (H _ eq_refl). auto.
-    - intros; destr. right. eapply public_stack_range_lo_ge_hi. omega.
   Qed.
 
 Lemma in_stack_tl:
@@ -1740,16 +1493,6 @@ Proof.
   destruct l; simpl; auto.
   intros; rewrite in_stack_cons; auto.
 Qed.
-
-
-(* Lemma in_frames_tl: *)
-(*   forall l b, *)
-(*     in_frames ((tl l)) b -> *)
-(*     in_frames (l) b. *)
-(* Proof. *)
-(*   destruct l; simpl; auto. *)
-(*   intros; rewrite in_frames_cons; auto. *)
-(* Qed. *)
 
 Lemma Forall_tl:
   forall {A} P (l: list A),
@@ -1834,11 +1577,11 @@ Fixpoint in_stack_all (s: stack) b : Prop :=
   end.
 
 Lemma in_frames_in_frames_all:
-  forall s b,
-    in_frames s b ->
-    in_frames_all s b.
+  forall tf b,
+    in_frames tf b ->
+    in_frames_all tf b.
 Proof.
-  induction s; simpl; intros; eauto.
+  induction tf; simpl; intros; eauto.
   rewrite in_frames_cons in H. destruct H as (fa & EQ & IFR). red. subst. simpl. left; auto.
 Qed.
 
@@ -1893,14 +1636,14 @@ Qed.
 
 Lemma stack_inject_aux_invariant:
   forall (m m': perm_type) f g s1 s2,
-    stack_inject_aux f m g s1 s2 ->
+    stack_inject f m g s1 s2 ->
     (forall b ofs k p,
         in_stack_all s1 b ->
         m' b ofs k p -> m b ofs k p) ->
-    stack_inject_aux f m' g s1 s2.
+    stack_inject f m' g s1 s2.
 Proof.
   induction 1; simpl; intros PERM; econstructor; eauto.
-  - eapply IHstack_inject_aux; eauto. subst.
+  - eapply IHstack_inject; eauto. subst.
     intros; eapply PERM; eauto using in_stack_all_drop.
   - eapply Forall_impl. 2: apply FI.
     simpl.
@@ -1914,52 +1657,21 @@ Lemma stack_inject_invariant:
   forall (m m': perm_type) f g s1 s2,
     (forall b ofs k p,
         in_stack_all s1 b ->
-        m' b ofs k p -> m b ofs k p) ->
-    (forall b1 b2 delta, f b1 = Some (b2, delta) ->
-                    ~ in_stack s1 b1 ->
-                    forall fi,
-                      in_stack' s2 (b2,fi) ->
-                      forall o k pp,
-                        m' b1 o k pp ->
-                        inject_perm_condition pp ->
-                        frame_public fi (o + delta)) ->
-    stack_inject f g m s1 s2 ->
-    stack_inject f g m' s1 s2.
+        m' b ofs k p -> m b ofs k p) -> (* just removed stuff here *)
+    stack_inject f m  g s1 s2 ->
+    stack_inject f m' g s1 s2.
 Proof.
-  intros m m' f g s1 s2 PERM PLT FI.
-  destruct FI. constructor; auto.
-  - intros.
+    intros.
     eapply stack_inject_aux_invariant; eauto.
-  - intros. eauto.
 Qed.
-
-  (* Lemma stack_inject_invariant': *)
-  (*   forall (m m': perm_type) f g f1 f2 thr, *)
-  (*     (forall b ofs k p, *)
-  (*         Plt b thr -> *)
-  (*         m' b ofs k p -> m b ofs k p) -> *)
-  (*     Forall (fun f1 => forall b, in_frames f1 b -> Plt b thr) f1 -> *)
-  (*     Forall (fun t1 => forall f1 b, In f1 (snd t1) -> in_frame f1 b -> Plt b thr) f1 -> *)
-  (*     (forall b1 b2 delta, f b1 = Some (b2, delta) -> *)
-  (*                     in_stack f2 b2 -> *)
-  (*                     Plt b1 thr) -> *)
-  (*     stack_inject f g m f1 f2 -> *)
-  (*     stack_inject f g m' f1 f2. *)
-  (* Proof. *)
-  (*   intros. *)
-  (*   eapply stack_inject_invariant; eauto. *)
-  (*   intros. *)
-  (*   elim H5. eapply H2; eauto. *)
-  (*   eapply in_stack'_in_stack; eauto. *)
-  (* Qed. *)
 
   Lemma stack_inject_aux_invariant_strong:
     forall (m m': perm_type) f g s1 s2,
-      stack_inject_aux f m g s1 s2 ->
+      stack_inject f m g s1 s2 ->
       (forall b ofs k p b' delta,
           f b = Some (b', delta) ->
           m' b ofs k p -> m b ofs k p) ->
-      stack_inject_aux f m' g s1 s2.
+      stack_inject f m' g s1 s2.
   Proof.
     induction 1; simpl; intros PERM; econstructor; eauto.
     eapply Forall_impl. 2: apply FI.
@@ -1968,24 +1680,21 @@ Qed.
   Qed.
 
   Lemma stack_inject_invariant_strong:
-    forall (m m': block -> _ -> _ -> _ -> Prop) f g f1 f2,
+    forall (m m': perm_type) f g f1 f2,
       (forall b ofs k p b' delta,
           f b = Some (b', delta) ->
           m' b ofs k p -> m b ofs k p) ->
-      stack_inject f g m f1 f2 ->
-      stack_inject f g m' f1 f2.
+      stack_inject f m  g f1 f2 ->
+      stack_inject f m' g f1 f2.
   Proof.
-    intros m m' f g f1 f2 PERM FI.
-    destruct FI. constructor; auto.
-    - intros. eapply stack_inject_aux_invariant_strong; eauto.
-    - intros; eapply stack_inject_not_in_source0; eauto.
+    intros. eapply stack_inject_aux_invariant_strong; eauto.
   Qed.
 
   Lemma stack_inject_nil:
     forall f p,
-      stack_inject f nil p nil nil.
+      stack_inject f p nil nil nil.
   Proof.
-    repeat constructor. easy.
+    repeat constructor.
   Qed.
 
   Lemma stack_inject_length_stack:
@@ -1994,12 +1703,11 @@ Qed.
       (length s2 <= length s1)%nat.
   Proof.
     intros j g P s1 s2 SI.
-    inversion SI.
-    revert stack_inject_frame_inject0. clear.
+    revert SI. clear.
     revert g s1 s2.
     induction 1; simpl; intros; eauto.
     simpl in *. repeat destr_in TAKE. simpl.
-    simpl in *. apply le_n_S. etransitivity. apply IHstack_inject_frame_inject0.
+    simpl in *. apply le_n_S. etransitivity. apply IHSI.
     rewrite drop_length. omega.
     eapply take_succeeds_inv; eauto.
   Qed.
@@ -2136,8 +1844,8 @@ Proof.
 Qed.
 
 Lemma size_frames_pos:
-  forall s,
-    (0 <= size_frames s)%Z.
+  forall tf,
+    (0 <= size_frames tf)%Z.
 Proof.
   intros. unfold size_frames. 
   apply Z.max_le_iff.
@@ -2240,7 +1948,7 @@ Qed.
 
   Lemma stack_inject_aux_id:
     forall p s,
-      stack_inject_aux inject_id p (flat_frameinj (length s)) s s.
+      stack_inject inject_id p (flat_frameinj (length s)) s s.
   Proof.
     induction s; simpl; intros; econstructor; simpl; eauto.
     repeat constructor.
@@ -2256,12 +1964,10 @@ Qed.
   Lemma stack_inject_id:
     forall p s,
       wf_stack p s ->
-      stack_inject inject_id (flat_frameinj (length s)) p s s.
+      stack_inject inject_id p (flat_frameinj (length s)) s s.
   Proof.
-    intros p s WF; constructor; auto.
+    intros p s WF; auto.
     eapply stack_inject_aux_id; eauto.
-    intros b1 b2 delta bi2 FB NIS FI o k p0 PERM IPC.
-    apply in_stack'_in_stack in FI. inv FB. congruence.
   Qed.
 
 (** The following shows how to transport a stack injection when more blocks get
@@ -2286,18 +1992,18 @@ allocated. *)
   Qed.
 
 Lemma stack_inject_aux_incr:
-  forall f f' g (p: block -> Z -> perm_kind -> permission -> Prop)  s1 s2,
-    stack_inject_aux f p g s1 s2 ->
+  forall f f' g (p: perm_type)  s1 s2,
+    stack_inject f p g s1 s2 ->
     inject_incr f f' ->
     (forall b b' delta,
         f b = None ->
         f' b = Some (b', delta) ->
         ~ in_stack s1 b) ->
-    stack_inject_aux f' p g s1 s2.
+    stack_inject f' p g s1 s2.
 Proof.
   induction 1; simpl; intros INCR NEW; econstructor; eauto.
   subst.
-  eapply IHstack_inject_aux; eauto.
+  eapply IHstack_inject; eauto.
   intros b b' delta H0 H1 INS. eapply NEW; eauto using in_stack_drop.
   eapply Forall_impl. 2: apply FI.
   simpl; intros.
@@ -2308,30 +2014,17 @@ Proof.
 Qed.
 
 Lemma stack_inject_incr:
-  forall f f' g (p: block -> Z -> perm_kind -> permission -> Prop)  s1 s2,
+  forall f f' g (p: perm_type)  s1 s2,
     inject_incr f f' ->
     (forall b b' delta,
         f b = None ->
         f' b = Some (b', delta) ->
-        ~ in_stack s1 b 
-        /\ forall fi,
-            in_stack' s2 (b', fi) ->
-            forall o k pp,
-              p b o k pp ->
-              inject_perm_condition pp ->
-              frame_public fi (o + delta)) ->
-    stack_inject f g p s1 s2 ->
-    stack_inject f' g p s1 s2.
+        ~ in_stack s1 b) ->
+    stack_inject f  p g s1 s2 ->
+    stack_inject f' p g s1 s2.
 Proof.
   intros f f' g p s1 s2 INCR NEW SI.
-  inversion SI; constructor; eauto.
-  - eapply stack_inject_aux_incr; eauto.
-    intros; eapply NEW; eauto.
-  - intros b1 b2 delta bi2 SOME NIS INS o k p0 P IPC.
-    destruct (f b1) as [[b2' delta']|] eqn:FB.
-    exploit INCR. eauto. rewrite SOME. inversion 1; subst.
-    eauto.
-    generalize (NEW _ _ _ FB SOME). intros (NIN1 & NIN2). eapply NIN2 in INS; eauto.
+  eapply stack_inject_aux_incr; eauto.
 Qed.
 
 Lemma norepet_1:
@@ -2358,12 +2051,12 @@ Definition make_singleton_frame_adt' (b: block) fi (sz: Z) :=
   |}.
 
   Lemma val_inject_ext:
-    forall j1 j2 m1 m2,
-      Val.inject j1 m1 m2 ->
+    forall j1 j2 v1 v2,
+      Val.inject j1 v1 v2 ->
       (forall x, j1 x = j2 x) ->
-      Val.inject j2 m1 m2.
+      Val.inject j2 v1 v2.
   Proof.
-    intros j1 j2 m1 m2 INJ EXT.
+    intros j1 j2 v1 v2 INJ EXT.
     inv INJ; econstructor; eauto.
     rewrite <- EXT; eauto.
   Qed.
@@ -2378,9 +2071,6 @@ Definition make_singleton_frame_adt' (b: block) fi (sz: Z) :=
     inv INJ; constructor; auto.
     eapply val_inject_ext; eauto.
   Qed.
-
-
-
 
 Lemma frame_inject_ext:
   forall j1 j2 f1 f2,
@@ -2419,9 +2109,9 @@ Qed.
 
   Lemma stack_inject_aux_ext':
     forall j1 j2 g P m1 m2,
-      stack_inject_aux j1 P g m1 m2 ->
-      (forall x, j1 x = j2 x) ->
-      stack_inject_aux j2 P g m1 m2.
+      stack_inject j1 P g m1 m2 ->
+      (forall b, j1 b = j2 b) ->
+      stack_inject j2 P g m1 m2.
   Proof.
     induction 1; simpl; intros; econstructor; eauto.
     eapply Forall_impl. 2: apply FI.
@@ -2431,25 +2121,22 @@ Qed.
 
   Lemma stack_inject_ext':
     forall j1 j2 g P m1 m2,
-      stack_inject j1 g P m1 m2 ->
-      (forall x, j1 x = j2 x) ->
-      stack_inject j2 g P m1 m2.
+      stack_inject j1 P g m1 m2 ->
+      (forall b, j1 b = j2 b) ->
+      stack_inject j2 P g m1 m2.
   Proof.
     intros j1 j2 g P m1 m2 INJ EXT.
-    inv INJ; constructor; eauto.
-    - eapply stack_inject_aux_ext'; eauto.
-    - intros.
-      eapply stack_inject_not_in_source0; eauto. rewrite EXT; eauto.
+    eapply stack_inject_aux_ext'; eauto.
   Qed.
 
 
-    Lemma frameinj_push_flat:
-      forall m,
-        flat_frameinj (Datatypes.S m) = 1%nat :: flat_frameinj m.
-    Proof.
-      reflexivity.
-    Qed.
-    
+  Lemma frameinj_push_flat:
+    forall m,
+      flat_frameinj (Datatypes.S m) = 1%nat :: flat_frameinj m.
+  Proof.
+    reflexivity.
+  Qed.
+
 Lemma frame_at_pos_cons:
   forall l i f a,
     frame_at_pos l i f ->
@@ -2510,34 +2197,24 @@ Inductive top_tframe_prop (P: tframe_adt -> Prop) : stack -> Prop :=
     P tf ->
     top_tframe_prop P (tf::r).
 
-
-(* Definition wf_tframe_strong (m: perm_type) (j: meminj) (f: tframe_adt) : Prop := *)
-(*   forall b, *)
-(*     j b <> None -> *)
-(*     in_frames f b -> *)
-(*     forall o k p, ~ m b o k p. *)
-
-
 Definition top_tframe_tc (s: stack) : Prop :=
   top_tframe_prop (fun tf => fst tf = None) s.
 
 Lemma stack_inject_push_new_stage_right:
   forall j n g P s1 s2,
-    stack_inject j (n :: g) P s1 s2 ->
+    stack_inject j P (n :: g) s1 s2 ->
     top_tframe_tc s1 ->
     (2 <= n)%nat ->
-    stack_inject j (1%nat :: pred n :: g) P s1 ((None,nil)::s2).
+    stack_inject j P (1%nat :: pred n :: g) s1 ((None,nil)::s2).
 Proof.
   intros j n g P s1 s2 SI TTNP Gof1.
-  inversion SI; constructor; auto.
-  - inv stack_inject_frame_inject0.
-    simpl in *. repeat destr_in TAKE.
-    econstructor. reflexivity. simpl. eauto.
-    destruct n0. omega. econstructor; eauto. inv FI; auto.
-    repeat constructor.
-    intros ff1 INf1 _. exfalso.
-    inv TTNP. congruence.
-  - simpl. intros; eapply stack_inject_not_in_source0; eauto. tauto.
+  inv SI.
+  simpl in *. repeat destr_in TAKE.
+  econstructor. reflexivity. simpl. eauto.
+  destruct n0. omega. econstructor; eauto. inv FI; auto.
+  repeat constructor.
+  intros ff1 INf1 _. exfalso.
+  inv TTNP. congruence.
 Qed.
 
 Lemma frame_at_pos_cons_inv:
@@ -2553,38 +2230,27 @@ Qed.
 
 Lemma stack_inject_unrecord_parallel:
   forall j g m1 s1 s2
-    (SI: stack_inject j (1%nat :: g) m1 s1 s2)
+    (SI: stack_inject j m1 (1%nat :: g) s1 s2)
     (ND2: nodup s2)
     fr2 l2
     (STK2 : s2 = fr2 :: l2)
     fr1 l1
     (STK1 : s1 = fr1 :: l1),
-    stack_inject j g m1 l1 l2.
+    stack_inject j m1 g l1 l2.
 Proof.
   intros. subst.
-  inversion SI; constructor; auto.
-  + inv stack_inject_frame_inject0. simpl in *; auto.
-  + simpl. intros b1 b2 delta bi2 JB NIS INS o k p PERM IPC.
-    inv stack_inject_frame_inject0. simpl in *; auto. inv TAKE.
-    inv FI. clear H2.
-    destruct (in_frames_dec fr1 b1).
-    * destruct (in_frames_in_frame_ex _ _ i) as (fr & INfrs & INFR).
-      inv ND2. edestruct H3.
-      eapply tframe_inject_in_frames; eauto.
-      eapply in_stack'_in_stack; eauto.
-    * eapply stack_inject_not_in_source0 in JB; eauto.
-      rewrite in_stack_cons. intuition.
+  inv SI. simpl in *; auto.
 Qed.
 
 Lemma stack_inject_unrecord_parallel_frameinj_flat_on:
   forall j m1 s1 s2
-    (SI: stack_inject j (flat_frameinj (length s2)) m1 s1 s2)
+    (SI: stack_inject j m1 (flat_frameinj (length s2)) s1 s2)
     (ND2: nodup s2)
     fr2 l2
     (STK2 : s2 = fr2 :: l2)
     fr1 l1
     (STK1 : s1 = fr1 :: l1),
-    stack_inject j (flat_frameinj (length l2)) m1 l1 l2.
+    stack_inject j m1 (flat_frameinj (length l2)) l1 l2.
 Proof.
   intros. subst.
   eapply stack_inject_unrecord_parallel; eauto.
@@ -2597,7 +2263,7 @@ Lemma same_sizes_frame_size_eq:
     same_sizes_frame f1 f2 ->
     size_frame f1 = size_frame f2.
 Proof.
-  intros f1 f2 SS; unfold size_frame; rewrite SS. reflexivity.
+  intros f1 f2 SS; unfold size_frame. rewrite SS. reflexivity.
 Qed.
 
 Definition same_sizes_list_frames tf1 tf2 :=
@@ -2709,73 +2375,6 @@ Program Definition inject_perm_all: InjectPerm :=
     inject_perm_condition := fun p => True
   |}.
 
-(* Definition same_head (P: perm_type) (m m': stack) := *)
-(*   list_forall2 *)
-(*     (fun tf1 tf2 => *)
-(*        (forall f1, In f1 tf1 -> has_perm_frame (injperm:=inject_perm_all) P inject_id f1 -> In f1 tf2) *)
-(*        /\ (forall f1, In f1 tf2 -> In f1 tf1) *)
-(*     ) *)
-(*     m m'. *)
-
-(* Lemma same_head_in_stack': *)
-(*   forall P s1 s2, same_head P s1 s2 -> forall b fi, in_stack' s2 (b,fi) -> in_stack' s1 (b,fi). *)
-(* Proof. *)
-(*   induction 1; simpl; intros; eauto. *)
-(*   destruct H. *)
-(*   destruct H1; auto. *)
-(*   left. *)
-(*   rewrite in_frames'_rew in H1. destruct H1 as (fr & IFR & INb1). *)
-(*   apply H2 in INb1. *)
-(*   rewrite in_frames'_rew; eauto. *)
-(* Qed. *)
-
-(* Lemma same_head_get_frame_info: *)
-(*   forall P s1 s2 (SH: same_head P s1 s2) *)
-(*     (ND: nodup s1) (ND': Forall nodupt s1) *)
-(*     b f (GFI: get_frame_info s2 b = Some f), *)
-(*     get_frame_info s1 b = Some f. *)
-(* Proof. *)
-(*   intros. *)
-(*   apply get_assoc_spec in GFI. *)
-(*   destruct GFI as (fr & tf & INblocks & INtf & INS). *)
-(*   exploit same_head_in_stack'; eauto. *)
-(*   rewrite in_stack'_rew. eexists; split; eauto. *)
-(*   rewrite in_frames'_rew. eexists; split; eauto. *)
-(*   intro INS'. *)
-(*   clear INblocks INtf INS. *)
-(*   rewrite in_stack'_rew in INS'. setoid_rewrite in_frames'_rew in INS'. *)
-(*   destruct INS' as (ttf & (tfr & IFR & ITF) & INS). *)
-(*   eapply get_assoc_stack_lnr; eauto. *)
-(* Qed. *)
-
-(* Lemma same_head_in_impl: *)
-(*   forall P s1 s2, same_head P s1 s2 -> forall b, in_stack s2 b -> in_stack s1 b. *)
-(* Proof. *)
-(*   intros. *)
-(*   eapply in_stack_in_frames_ex in H0. destruct H0 as (tf & INS & IFRS). *)
-(*   eapply in_frames_in_frame_ex in IFRS. destruct IFRS as (fr & IFRS & IFR). *)
-(*   apply in_frame_info in IFR. destruct IFR as (fi & IFR). *)
-(*   eapply in_stack'_in_stack. eapply same_head_in_stack'; eauto. *)
-(*   rewrite in_stack'_rew. eexists; split; eauto. *)
-(*   rewrite in_frames'_rew. eexists; split; eauto. *)
-(* Qed. *)
-
-(* Lemma same_head_fap: *)
-(*   forall P s1 s2 (SH: same_head P s1 s2) *)
-(*          f1 i (FAP1: f1 @ s1 : i), *)
-(*   exists f2, f2 @ s2 : i /\ (forall ff1, In ff1 f1 -> has_perm_frame (injperm:= inject_perm_all) P inject_id ff1 -> In ff1 f2). *)
-(* Proof. *)
-(*   induction 1; simpl; intros; eauto. *)
-(*   destruct H. *)
-(*   destruct i. *)
-(*   - apply frame_at_pos_last in FAP1. subst. *)
-(*     exists b1; split. constructor; reflexivity. *)
-(*     auto. *)
-(*   - apply frame_at_pos_cons_inv in FAP1. *)
-(*     eapply IHSH in FAP1. destruct FAP1 as (f2 & FAP2 & PROP). *)
-(*     exists f2; split. apply frame_at_pos_cons. auto. eauto. omega. *)
-(* Qed. *)
-
 Lemma has_perm_frame_impl {injperm: InjectPerm}:
   forall (P1 P2: perm_type) j f tf,
     has_perm_frame P1 j f ->
@@ -2795,80 +2394,8 @@ Proof.
   split. eapply in_frame'_in_frame; eauto. split; eauto.
 Qed.
 
-(* Lemma same_head_more_perm {injperm: InjectPerm}: *)
-(*   forall (P1 P2: perm_type) s1 s2 *)
-(*          (SH: same_head P1 s1 s2) *)
-(*          (SAMEPERM: forall b o k p, in_stack s1 b -> P2 b o k p -> P1 b o k p), *)
-(*     same_head P2 s1 s2. *)
-(* Proof. *)
-(*   induction 1; simpl; intros; constructor; auto. *)
-(*   - destruct H; split; auto. *)
-(*     intros; eapply H; eauto. *)
-(*     destruct H2 as (b & o & k & p & NONE & IFR & PERM & IPC). *)
-(*     exists b, o, k, p; repeat split; eauto. eapply SAMEPERM; eauto. *)
-(*     rewrite in_stack_cons; left. *)
-(*     eapply in_frame_in_frames; eauto. *)
-(*   - apply IHSH. intros. eapply SAMEPERM; eauto. *)
-(*     apply in_stack_tl. simpl; auto. *)
-(* Qed. *)
-
-(* Lemma public_stack_access_same_head: *)
-(*   forall s1 (ND: nodup s1) (ND': Forall nodupt s1) s2 P (SH: same_head P s1 s2) b lo hi *)
-(*          (PSA: public_stack_access s1 b lo hi), *)
-(*     public_stack_access s2 b lo hi. *)
-(* Proof. *)
-(*   intros. red. destr. red in PSA. *)
-(*   erewrite same_head_get_frame_info in PSA; eauto. *)
-(* Qed. *)
-
 Definition stack_top_is_new s :=
   top_tframe_prop (fun tf => tf = (None,nil)) s.
-
-(* Lemma is_stack_top_same_head: *)
-(*   forall P s1 (WF: wf_stack P inject_id s1) (ND: nodup s1) s2 (SH: same_head P s1 s2) b *)
-(*          o k p (PERM: P b o k p) *)
-(*          (IST: is_stack_top s1 b), *)
-(*     is_stack_top s2 b \/ ~ in_stack s2 b. *)
-(* Proof. *)
-(*   intros. *)
-(*   inv SH. easy. *)
-(*   destruct H. *)
-(*   red in IST. simpl in IST. *)
-(*   change (in_frames a1 b) in IST. *)
-(*   left. red. simpl. *)
-(*   change (in_frames b1 b). *)
-(*   edestruct in_frames_in_frame_ex as (fr & IFRS & IFR). eauto. *)
-(*   eapply in_frame_in_frames; eauto. apply H; auto. *)
-(*   exists b, o, k, p; repeat split; auto. unfold inject_id; congruence. *)
-(* Qed. *)
-
-(* Lemma stack_access_same_head: *)
-(*   forall s1 P (ND: nodup s1) (ND': Forall nodupt s1) (WF: wf_stack P inject_id s1) s2 (SH: same_head P s1 s2) b lo hi k p *)
-(*          (R: forall o, (lo <= o < hi)%Z -> P b o k p) *)
-(*          (SA: stack_access s1 b lo hi), *)
-(*     stack_access s2 b lo hi. *)
-(* Proof. *)
-(*   intros. *)
-(*   destruct (zlt lo hi). *)
-(*   destruct SA as [IST|PSA]. *)
-(*   edestruct is_stack_top_same_head; eauto. apply (R lo). omega. left; auto. *)
-(*   right; red; destr. eapply get_frame_info_in_stack in Heqo; congruence. *)
-(*   right; eapply public_stack_access_same_head; eauto. *)
-(*   eapply lo_ge_hi_stack_access; eauto. *)
-(* Qed. *)
-
-(* Lemma stack_access_same_head_or_not_in_stack: *)
-(*   forall s1 P (ND: nodup s1) (ND': Forall nodupt s1) (WF: wf_stack P inject_id s1) s2 b *)
-(*          (SH: same_head P s1 s2 \/ ~ in_stack s2 b) lo hi k p *)
-(*          (R: forall o, (lo <= o < hi)%Z -> P b o k p) *)
-(*          (SA: stack_access s1 b lo hi), *)
-(*     stack_access s2 b lo hi. *)
-(* Proof. *)
-(*   intros. *)
-(*   destruct SH as [SH | NIS]. *)
-(*   eapply stack_access_same_head; eauto. *)
-(*   right. red. destr. apply get_frame_info_in_stack in Heqo. congruence.           *)
-(* Qed. *)
 
 Lemma max_in_le:
   forall l a i,
@@ -2892,24 +2419,6 @@ Proof.
   apply max_in_le; auto.
   apply IHl1. auto.
 Qed.
-
-(* Lemma same_head_size: *)
-(*   forall P s1 s2, *)
-(*     same_head P s1 s2 -> *)
-(*     (size_stack s2 <= size_stack s1)%Z. *)
-(* Proof. *)
-(*   induction 1; simpl; intros; rewrite ? size_stack_cons. omega. *)
-(*   cut (size_frames b1 <= size_frames a1)%Z. omega. *)
-(*   apply max_sublist. setoid_rewrite in_map_iff. *)
-(*   intros x (x0 & EQ & IN). exists x0; split; auto. apply H. auto. *)
-(* Qed. *)
-
-(* Lemma same_head_refl: *)
-(*   forall P s, *)
-(*     same_head P s s. *)
-(* Proof. *)
-(*   induction s; simpl; intros; constructor; eauto. *)
-(* Qed. *)
 
 (* For use in Mach and Asm, the parent_sp pointer is now computed on the stack
    adt rather than on the abstract semantic callstack in Mach or with an extra
@@ -2944,6 +2453,7 @@ Proof.
   unfold parent_sp, current_sp, current_frame_sp. intros.
   repeat destr; try now (simpl; auto).
 Qed.
+
 Definition opt_cons {A: Type} (o: option A) (l: list A) : list A :=
   match o with
     None => l
